Starting the hybrid simulation proofs.

concurrency/compiler/concurrent_compiler_simulation_proof.v
@@ -4,6 +4,71 @@ Require Import VST.concurrency.compiler.concurrent_compiler_simulation.
 Require Import VST.concurrency.compiler.sequential_compiler_correct.
 
 
+(*
+(*Clight Machine *)
+Require Import VST.concurrency.common.ClightMachine.
+(*Asm Machine*)
+Require Import VST.concurrency.common.x86_context.
+
+
+(** *One thread simulation*)
+Module OneThreadSimulation (CC_correct: CompCert_correctness).
+  
+  Import HybridMachineSig.
+
+  Module DMS.
+  Section DMS.
+
+  Existing Instance OrdinalPool.OrdinalThreadPool.
+  Context (Clight_g : Clight.genv).
+  Definition CSem : Semantics := ClightSemantincsForMachines.ClightSem Clight_g.
+  
+  Import X86Context.
+
+  (*Import the Asm Hybrid Machine*)
+  Context (Asm_g : Clight.genv).
+  Context (Asm_program: Asm.program).
+  Context (Asm_genv_safe: Asm_core.safe_genv (@the_ge Asm_program)).
+
+  
+  Definition AsmSem : Semantics := @X86Sem Asm_program Asm_genv_safe.
+
+  
+
+  (* First construct the Clight machine and the two projections:
+     - ClightMachineSem (i.e.  MachineSemantics) 
+     - ClightConcurSem (i.e. ConcurMachineSemantics)
+  *)
+  
+  Definition ClightMachine :=(HybridCoarseMachine.HybridCoarseMachine
+                                 (machineSig := DryHybridMachine.DryHybridMachineSig)).
+  Definition ClightMachineSem := (MachineSemantics(HybridMachine := ClightMachine)).
+  Definition ClightConcurSem := (ConcurMachineSemantics(HybridMachine := ClightMachine)). 
+  
+
+  
+  Lemma compile_one_thread:
+    
+    HybridMachine_simulation.HybridMachine_simulation
+  
+  
+  Lemma ConcurrentCompilerCorrectness:
+    forall (p:Clight.program) (tp:Asm.program),
+      CC_correct.CompCert_compiler p = Some tp ->
+      forall asm_genv_safety,
+        ConcurrentCompilerCorrectness_specification
+          (Clight.globalenv p) tp asm_genv_safety
+          (Genv.init_mem (Ctypes.program_of_program p)) (Genv.init_mem tp)
+  .
+  Proof.
+    unfold ConcurrentCompilerCorrectness_specification.
+    intros.
+    apply CC_correct.simpl_clight_semantic_preservation in H.
+    unfold ClightMachine.ClightMachine.DMS.ClightConcurSem, HybridMachineSig.HybridMachineSig.ConcurMachineSemantics, ClightMachine.ClightMachine.DMS.ClightMachine, HybridMachineSig.HybridMachineSig.HybridCoarseMachine.HybridCoarseMachine.
+    econstructor.
+*)
+
+
 Module Concurrent_correctness (CC_correct: CompCert_correctness).
 
   
@@ -18,8 +83,8 @@ Module Concurrent_correctness (CC_correct: CompCert_correctness).
   Proof.
     unfold ConcurrentCompilerCorrectness_specification.
     intros.
+    apply CC_correct.simpl_clight_semantic_preservation in H.
     unfold ClightMachine.ClightMachine.DMS.ClightConcurSem, HybridMachineSig.HybridMachineSig.ConcurMachineSemantics, ClightMachine.ClightMachine.DMS.ClightMachine, HybridMachineSig.HybridMachineSig.HybridCoarseMachine.HybridCoarseMachine.
-    eapply CC_correct.simpl_clight_semantic_preservation in H.
     econstructor.
     
   Admitted.
